\subsection{3.2.19}

Пусть $\vec a=4\vec i-\vec j-2\vec k$, то есть $\vec a=(4;-1;-2)$, и $\vec b=(2;1;2)$. Тогда
\begin{gather*}
\vec a\cdot\vec b=4\cdot2+(-1)\cdot1+(-2)\cdot2=3, \\
a=\sqrt{4^2+(-1)^2+(-2)^2}=\sqrt{21}, \\
b=\sqrt{2^2+1^2+2^2}=3,
\end{gather*}
а значит,
\begin{gather*}
\left(\widehat{\vec a,\vec b}\right)=\arccos\frac{\vec a\cdot\vec b}{a\cdot b}=\arccos\frac{\sqrt{21}}{21}, \\
\text{ПР}_{\vec a}\vec b=b\cos\left(\widehat{\vec a,\vec b}\right)=\frac{\vec a\cdot\vec b}{a}=\frac{\sqrt{21}}{7}, \\
\text{ПР}_{\vec b}\vec a=a\cos\left(\widehat{\vec a,\vec b}\right)=\frac{\vec a\cdot\vec b}{b}=1.
\end{gather*}
